test/Ctypes1.fst
@@ -3,7 +3,6 @@ module Ctypes1
 open FStar.Mul
 open FStar.UInt
 module U32 = FStar.UInt32
-module U128 = FStar.UInt128
 
 type point = { x: U32.t; y: U32.t }
 
